value_of with steps

ch7/app/checkedlang/rocq/Interp.v
@@ -12,57 +12,73 @@ Module Import EnvNS := Env.
 Open Scope string_scope.
 Open Scope Z_scope.
 
-Local Unset Guard Checking.
+Inductive EvalResult : Type :=
+| EvalValue (val : ExpVal)
+| EvalRuntimeError
+| EvalGasExhausted.
 
-Definition bind_option {A B : Type} (oa : option A) (k : A -> option B) : option B :=
-  match oa with
-  | Some a => k a
-  | None => None
+Definition bind_eval (r : EvalResult) (k : ExpVal -> EvalResult) : EvalResult :=
+  match r with
+  | EvalValue v => k v
+  | EvalRuntimeError => EvalRuntimeError
+  | EvalGasExhausted => EvalGasExhausted
   end.
 
-Fixpoint value_of (exp : Exp) (env : Env) {struct exp} : option ExpVal :=
-  match exp with
-  | Const_Exp n => Some (Num_Val n)
-  | Var_Exp var => apply_env env var
-  | Diff_Exp e1 e2 =>
-      bind_option (value_of e1 env) (fun v1 =>
-      bind_option (value_of e2 env) (fun v2 =>
-        match v1, v2 with
-        | Num_Val n1, Num_Val n2 => Some (Num_Val (n1 - n2))
-        | _, _ => None
-        end))
-  | IsZero_Exp e =>
-      bind_option (value_of e env) (fun v =>
-        match v with
-        | Num_Val n => Some (Bool_Val (Z.eqb n 0))
-        | _ => None
-        end)
-  | If_Exp cond_exp then_exp else_exp =>
-      bind_option (value_of cond_exp env) (fun v =>
-        match v with
-        | Bool_Val true => value_of then_exp env
-        | Bool_Val false => value_of else_exp env
-        | _ => None
-        end)
-  | Let_Exp var exp1 body =>
-      bind_option (value_of exp1 env) (fun val1 =>
-        value_of body (extend_env var val1 env))
-  | Letrec_Exp _ proc_name bound_var _ proc_body letrec_body =>
-      value_of letrec_body (extend_env_rec proc_name bound_var proc_body env)
-  | Proc_Exp var _ body =>
-      Some (Proc_Val (procedure var body env))
-  | Call_Exp rator rand =>
-      bind_option (value_of rator env) (fun proc_val =>
-      bind_option (value_of rand env) (fun arg_val =>
-        match proc_val with
-        | Proc_Val p => apply_procedure p arg_val
-        | _ => None
-        end))
+Fixpoint value_of (step : nat) (exp : Exp) (env : Env) {struct step} : EvalResult :=
+  match step with
+  | O => EvalGasExhausted
+  | S step' =>
+      match exp with
+      | Const_Exp n => EvalValue (Num_Val n)
+      | Var_Exp var =>
+          match apply_env env var with
+          | Some v => EvalValue v
+          | None => EvalRuntimeError
+          end
+      | Diff_Exp e1 e2 =>
+          bind_eval (value_of step' e1 env) (fun v1 =>
+          bind_eval (value_of step' e2 env) (fun v2 =>
+            match v1, v2 with
+            | Num_Val n1, Num_Val n2 => EvalValue (Num_Val (n1 - n2))
+            | _, _ => EvalRuntimeError
+            end))
+      | IsZero_Exp e =>
+          bind_eval (value_of step' e env) (fun v =>
+            match v with
+            | Num_Val n => EvalValue (Bool_Val (Z.eqb n 0))
+            | _ => EvalRuntimeError
+            end)
+      | If_Exp cond_exp then_exp else_exp =>
+          bind_eval (value_of step' cond_exp env) (fun v =>
+            match v with
+            | Bool_Val true => value_of step' then_exp env
+            | Bool_Val false => value_of step' else_exp env
+            | _ => EvalRuntimeError
+            end)
+      | Let_Exp var exp1 body =>
+          bind_eval (value_of step' exp1 env) (fun val1 =>
+            value_of step' body (extend_env var val1 env))
+      | Letrec_Exp _ proc_name bound_var _ proc_body letrec_body =>
+          value_of step' letrec_body (extend_env_rec proc_name bound_var proc_body env)
+      | Proc_Exp var _ body =>
+          EvalValue (Proc_Val (procedure var body env))
+      | Call_Exp rator rand =>
+          bind_eval (value_of step' rator env) (fun proc_val =>
+          bind_eval (value_of step' rand env) (fun arg_val =>
+            match proc_val with
+            | Proc_Val p => apply_procedure step' p arg_val
+            | _ => EvalRuntimeError
+            end))
+      end
   end
-with apply_procedure (proc : Proc) (arg : ExpVal) {struct proc} : option ExpVal :=
-  match proc with
-  | Procedure var body saved_env =>
-      value_of body (extend_env var arg saved_env)
+with apply_procedure (step : nat) (proc : Proc) (arg : ExpVal) {struct step} : EvalResult :=
+  match step with
+  | O => EvalGasExhausted
+  | S step' =>
+      match proc with
+      | Procedure var body saved_env =>
+          value_of step' body (extend_env var arg saved_env)
+      end
   end.
 
 Definition initEnv : Env :=
@@ -70,12 +86,11 @@ Definition initEnv : Env :=
     (extend_env "v" (Num_Val 5)
       (extend_env "x" (Num_Val 10) empty_env)).
 
-Definition value_of_program (exp : Exp) : option ExpVal :=
-  value_of exp initEnv.
+Definition value_of_program (step : nat) (exp : Exp) : EvalResult :=
+  value_of step exp initEnv.
 
 End Interp.
 
 Export Interp.
 
-Set Guard Checking.
 Set Warnings "+masking-absolute-name".
