ch7/app/checkedlang/rocq/TypeSound.v
@@ -129,12 +129,12 @@ Proof.
   repeat constructor; constructor.
 Qed.
 
-Lemma bind_option_some :
-  forall (A B : Type) (oa : option A) (k : A -> option B) b,
-    bind_option oa k = Some b ->
-    exists a, oa = Some a /\n+              k a = Some b.
+Lemma bind_eval_value :
+  forall r k v,
+    bind_eval r k = EvalValue v ->
+    exists x, r = EvalValue x /\ k x = EvalValue v.
 Proof.
-  intros A B [a|] k b H;
+  intros [val| |] k v H;
     simpl in H;
     try discriminate.
   eauto.
@@ -143,7 +143,7 @@ Qed.
 Lemma bind_inr :
   forall (r : TyResult) (k : Ty -> TyResult) ty,
     bind r k = inr ty ->
-    exists v, r = inr v /
+    exists v, r = inr v /\
               k v = inr ty.
 Proof.
   intros [err|v] k ty H;
@@ -152,63 +152,167 @@ Proof.
   - eauto.
 Qed.
 
+Lemma type_sound_mutual :
+  forall step,
+    (forall exp env tenv ty val,
+        env_has_type env tenv ->
+        type_of exp tenv = inr ty ->
+        value_of step exp env = EvalValue val ->
+        value_has_type val ty)
+    /\
+    (forall proc arg val argTy resultTy,
+        value_has_type (Proc_Val proc) (TyFun argTy resultTy) ->
+        value_has_type arg argTy ->
+        apply_procedure step proc arg = EvalValue val ->
+        value_has_type val resultTy).
+Proof.
+  induction step as [|step IH].
+  - split.
+    + intros exp env tenv ty val _ _ Heval.
+      simpl in Heval.
+      discriminate.
+    + intros proc arg val argTy resultTy _ _ Happ.
+      simpl in Happ.
+      destruct proc; discriminate.
+  - destruct IH as [IHenv IHproc].
+    split.
+    + intros exp env tenv ty val Henv Hty Heval.
+      simpl in Heval.
+      destruct exp as
+          [n
+          | e1 e2
+          | e
+          | cond_exp then_exp else_exp
+          | id
+          | var exp1 body
+          | result_ty proc_name bound_var bound_ty proc_body letrec_body
+          | param param_ty body_proc
+          | rator rand]; simpl in *.
+      * inversion Hty; inversion Heval; constructor.
+      * destruct (apply_env env id) eqn:Hlookup; inversion Heval; subst.
+        eapply env_lookup_sound; eauto.
+      * apply bind_inr in Hty as [ty1 [Hty1 Hty]].
+        apply bind_inr in Hty as [ty2 [Hty2 Hty]].
+        destruct ty1; try (simpl in Hty; discriminate).
+        destruct ty2; try (simpl in Hty; discriminate).
+        inversion Hty; subst ty.
+        simpl in Heval.
+        apply bind_eval_value in Heval as [v1 [Heval1 Heval]].
+        apply bind_eval_value in Heval as [v2 [Heval2 Heval]].
+        pose proof (IHenv _ _ _ _ _ Henv Hty1 Heval1) as Hv1_ty.
+        pose proof (IHenv _ _ _ _ _ Henv Hty2 Heval2) as Hv2_ty.
+        inversion Hv1_ty; subst.
+        inversion Hv2_ty; subst.
+        inversion Heval; subst.
+        constructor.
+      * apply bind_inr in Hty as [ty1 [Hty1 Hty]].
+        destruct ty1; try (simpl in Hty; discriminate).
+        inversion Hty; subst ty.
+        simpl in Heval.
+        apply bind_eval_value in Heval as [v [Heval1 Heval]].
+        pose proof (IHenv _ _ _ _ _ Henv Hty1 Heval1) as Hv_ty.
+        inversion Hv_ty; subst.
+        simpl in Heval.
+        inversion Heval; subst.
+        constructor.
+      * apply bind_inr in Hty as [condTy [HcondTy Hty]].
+        destruct condTy; try (simpl in Hty; discriminate).
+        apply bind_inr in Hty as [thenTy [HthenTy Hty]].
+        apply bind_inr in Hty as [elseTy [HelseTy Hty]].
+        destruct (equal_ty thenTy elseTy) eqn:Heq; try (simpl in Hty; discriminate).
+        simpl in Hty.
+        inversion Hty; subst ty.
+        apply equal_ty_eq in Heq; subst elseTy.
+        simpl in Heval.
+        apply bind_eval_value in Heval as [cond_val [Hcond Heval]].
+        pose proof (IHenv _ _ _ _ _ Henv HcondTy Hcond) as Hcond_typed.
+        inversion Hcond_typed; subst.
+        destruct b.
+        -- simpl in Heval.
+           eapply IHenv; eauto.
+        -- simpl in Heval.
+           eapply IHenv; eauto.
+      * apply bind_inr in Hty as [expTy [HexpTy Hty]].
+        simpl in Heval.
+        apply bind_eval_value in Heval as [val1 [Hval1 Heval]].
+        pose proof (IHenv _ _ _ _ _ Henv HexpTy Hval1) as Hval1_ty.
+        pose proof (env_extend_has_type _ _ _ _ _ Henv Hval1_ty) as Henv_ext.
+        eapply IHenv with (exp := body)
+                          (env := extend_env var val1 env)
+                          (tenv := extend_tyenv var expTy tenv)
+                          (ty := ty);
+          eauto.
+      * apply bind_inr in Hty as [procbodyTy [HprocTy Hty]].
+        destruct (equal_ty result_ty procbodyTy) eqn:Heq; try (simpl in Hty; discriminate).
+        simpl in Hty.
+        apply equal_ty_eq in Heq; subst procbodyTy.
+        pose proof (env_has_type_extend_rec_preserves _ _ _ _ _ _ _ Henv HprocTy) as Henv_rec.
+        eapply IHenv with (exp := letrec_body)
+                          (env := extend_env_rec proc_name bound_var proc_body env)
+                          (tenv := extend_tyenv proc_name (TyFun bound_ty result_ty) tenv)
+                          (ty := ty);
+          eauto.
+      * apply bind_inr in Hty as [bodyTy [HbodyTy Hty]].
+        inversion Hty; subst ty.
+        inversion Heval; subst.
+        eapply value_has_type_proc_intro; eauto.
+      apply bind_inr in Hty as [funTy [HfunTy Hty]].
+      apply bind_inr in Hty as [argTy [HargTy Hty]].
+        destruct funTy; try (simpl in Hty; discriminate).
+        destruct (equal_ty dom argTy) eqn:Heq; try (simpl in Hty; discriminate).
+        simpl in Hty.
+        inversion Hty; subst ty.
+        simpl in Heval.
+        apply bind_eval_value in Heval as [proc_val [Hproc Heval]].
+        apply bind_eval_value in Heval as [arg_val [Harg Heval]].
+        pose proof (IHenv _ _ _ _ _ Henv HfunTy Hproc) as Hproc_ty.
+        pose proof (IHenv _ _ _ _ _ Henv HargTy Harg) as Harg_ty.
+        apply equal_ty_eq in Heq; subst argTy.
+      destruct proc_val as [n|b|p]; simpl in Heval; try discriminate.
+      eapply IHproc; eauto.
+    + intros proc arg val argTy resultTy Hproc Harg Happ.
+      destruct proc as [param body saved_env].
+      simpl in Happ.
+      inversion Hproc as [ | | param' body' saved_env' tenv' argTy' resultTy' Henv_saved HbodyTy]; subst.
+      pose proof (env_extend_has_type _ _ _ _ _ Henv_saved Harg) as Henv_ext.
+      eapply IHenv with (exp := body)
+                        (env := extend_env param arg saved_env)
+                        (tenv := extend_tyenv param argTy tenv')
+                        (ty := resultTy);
+        eauto.
+Qed.
+
 Lemma type_sound_env :
-  forall exp env tenv ty val,
+  forall step exp env tenv ty val,
     env_has_type env tenv ->
     type_of exp tenv = inr ty ->
-    value_of exp env = Some val ->
-    value_has_type val ty
-with type_sound_proc :
-  forall proc arg val argTy resultTy,
-    value_has_type (Proc_Val proc) (TyFun argTy resultTy) ->
-    value_has_type arg argTy ->
-    apply_procedure proc arg = Some val ->
-    value_has_type val resultTy.
-Proof.
-  - intros exp env tenv ty val Henv Hty Hval.
-    revert env tenv ty val Henv Hty Hval.
-    induction exp; intros env tenv ty val Henv Hty Hval; simpl in *.
-    + inversion Hty; inversion Hval; constructor.
-    + (* Diff_Exp *)
-      apply bind_inr in Hty as [ty1 [Hty1 Hty]].
-      apply bind_inr in Hty as [ty2 [Hty2 Hty]].
-      destruct ty1; try (simpl in Hty; discriminate).
-      destruct ty2; try (simpl in Hty; discriminate).
-      inversion Hty; subst ty.
-      apply bind_option_some in Hval as [v1 [Hv1 Hval]].
-      apply bind_option_some in Hval as [v2 [Hv2 Hval]].
-      destruct v1; try discriminate.
-      destruct v2; try discriminate.
-      inversion Hval; subst val.
-      pose proof (IHexp1 env tenv TyInt (Num_Val n) Henv Hty1 Hv1) as Hv1_ty.
-      pose proof (IHexp2 env tenv TyInt (Num_Val n0) Henv Hty2 Hv2) as Hv2_ty.
-      inversion Hv1_ty; subst.
-      inversion Hv2_ty; subst.
-      constructor.
-    + (* IsZero_Exp *)
-      apply bind_option_some in Hval as [v [Hv Hval]].
-      destruct v; try discriminate.
-      inversion Hval; subst.
-      apply bind_inr in Hty as [ty1 [Hty1 Hty]].
-      destruct ty1; try (simpl in Hty; discriminate).
-      inversion Hty; subst ty.
-      pose proof (IHexp env tenv TyInt (Num_Val n) Henv Hty1 Hv) as Hv_ty.
-      inversion Hv_ty; subst.
-      constructor.
-    + (* If_Exp *)
-      apply bind_inr in Hty as [condTy [HcondTy Hty]].
-      destruct condTy; try (simpl in Hty; discriminate).
-      apply bind_inr in Hty as [thenTy [HthenTy Hty]].
-      destruct (equal_ty thenTy (let '(If_Exp _ _ _) := If_Exp exp1 exp2 exp3 in exp3) ); simpl in Hty.
-Abort.
-
-Theorem type_sound :
-  forall (exp : Exp) (ty : Ty) (val : ExpVal),
-    type_of_program exp = inr ty ->
-    value_of_program exp = Some val ->
+    value_of step exp env = EvalValue val ->
     value_has_type val ty.
 Proof.
-  intros exp ty val Htyped Heval.
+  intros step exp env tenv ty val Henv Hty Heval.
+  destruct (type_sound_mutual step) as [H _].
+  eapply H; eauto.
+Qed.
+
+Lemma type_sound_proc :
+  forall step proc arg val argTy resultTy,
+    value_has_type (Proc_Val proc) (TyFun argTy resultTy) ->
+    value_has_type arg argTy ->
+    apply_procedure step proc arg = EvalValue val ->
+    value_has_type val resultTy.
+Proof.
+  intros step proc arg val argTy resultTy Hproc Harg Happ.
+  destruct (type_sound_mutual step) as [_ H].
+  eapply H; eauto.
+Qed.
+
+Theorem type_sound :
+  forall (step : nat) (exp : Exp) (ty : Ty) (val : ExpVal),
+    type_of_program exp = inr ty ->
+    value_of_program step exp = EvalValue val ->
+    value_has_type val ty.
+Proof.
+  intros step exp ty val Htyped Heval.
   unfold type_of_program in Htyped.
   unfold value_of_program in Heval.
   eapply type_sound_env; eauto.
